Coq/Software Foundation/Q_hoare.v
@@ -1,0 +1,118 @@
+(*
+  contents:
+  1. Assertion
+    - Open Scope XX
+  2. Hoare Triples
+  3.
+  4.
+  5.
+*)
+
+Require Import Coq.Bool.Bool.
+Require Import Coq.Arith.Arith.
+Require Import Coq.Arith.EqNat.
+Require Import Coq.omega.Omega.
+Require Import Coq.Lists.List.
+Require Import Coq.Logic.FunctionalExtensionality.
+Import ListNotations.
+Require Import H_maps.
+Require Import L_imp.
+
+
+(*
+在equiv.v中我们讨论了imp的一些meta property。"meta" in the sense 
+that they are properties of the language as a whole, rather 
+than of particular programs in the language.
+
+在本章中将讲一个 systematic method for reasoning about the correctness
+of PARTICULAR programs in Imp
+*)
+
+
+
+(* Assertions *)
+(*------------------------------------------------------------*)
+(*
+an assertion is just a family of propositions indexed by a state.
+*)
+Definition Assertion := state -> Prop.
+
+(*example*)
+Module ExAssertions.
+
+Definition as1 : Assertion := fun st => st X = 3.
+Definition as2 : Assertion := fun st => st X <= st Y.
+Definition as3 : Assertion :=
+  fun st => st X = 3 \/ st X <= st Y.
+Definition as4 : Assertion :=
+  fun st => st Z * st Z <= st X /\
+            ~ (((S (st Z)) * (S (st Z))) <= st X).
+Definition as5 : Assertion := fun st => True.
+Definition as6 : Assertion := fun st => False.
+
+End ExAssertions.
+
+
+(*
+Given two assertions P and Q, we say that P implies Q, written 
+P ->> Q, if, whenever P holds in some state st, Q also holds.
+*)
+Definition assert_implies (P Q: Assertion) : Prop :=
+  forall st, P st -> Q st.
+
+Notation "P ->> Q" := (assert_implies P Q)
+                      (at level 80) : hoare_spec_scope.
+
+Open Scope hoare_spec_scope. 
+
+
+(* Open Scope XX *)
+(*
+The hoare_spec_scope annotation here tells Coq that this 
+notation is not global but is intended to be used in particular
+contexts. The Open Scope tells Coq that this file is one such 
+context.
+*)
+
+Notation "P <<->> Q" :=
+  (P ->> Q ∧ Q <<- P) (at level 80) : hoare_spec_scope.
+
+
+
+
+
+
+
+
+
+
+
+(* Hoare Triples *)
+(*------------------------------------------------------------*)
+
+
+
+
+
+
+
+
+
+
+
+
+
+
+
+
+
+
+
+
+
+
+
+
+(*------------------------------------------------------------*)
+(*------------------------------------------------------------*)
+(*------------------------------------------------------------*)
